pulse/lib/pulse/lib/Pulse.Lib.Slice.fsti
@@ -104,6 +104,13 @@ val split (#t: Type) (s: slice t) (#p: perm) (i: SZ.t) (#v: Ghost.erased (Seq.se
       pts_to s2 #p (Seq.slice v (SZ.v i) (Seq.length v)) **
       is_split s s1 s2)
 
+val ghost_split (#t: Type) (s: slice t) (#p: perm) (i: SZ.t) (#v: Ghost.erased (Seq.seq t) { SZ.v i <= Seq.length v }) : stt_ghost (Ghost.erased (slice t & slice t)) emp_inames
+    (requires pts_to s #p v)
+    (ensures fun res ->
+      pts_to (fst res) #p (Seq.slice v 0 (SZ.v i)) **
+      pts_to (snd res) #p (Seq.slice v (SZ.v i) (Seq.length v)) **
+      is_split s (fst res) (snd res))
+
 val join (#t: Type) (s1: slice t) (#p: perm) (#v1: Seq.seq t) (s2: slice t) (#v2: Seq.seq t) (s: slice t) : stt_ghost unit emp_inames
     (pts_to s1 #p v1 ** pts_to s2 #p v2 ** is_split s s1 s2)
     (fun _ -> pts_to s #p (Seq.append v1 v2))
